PKS, EF/UF-CMA and PSS from scratch. Starting OW. Beginning usage-guided abstraction of bitstrings and words.
DO NOT USE OW.EC for real proofs in its current state!

examples/PSS.ec
@@ -1,48 +1,123 @@
-require import Bitstring.
+require import Fun.
 require import Int.
-require import Distr.
 
-(* Protocol-specific constants *)
+(*** General definitions *)
+(** Lengths *)
 op k:int.
-axiom leq0_k: 0 <= k.
+axiom leq0_k: 0 < k.
+
 op k0:int.
-axiom leq0_k0: 0 <= k0.
+axiom leq0_k0: 0 < k0.
+
 op k1:int.
-axiom leq0_k1: 0 <= k1.
+axiom leq0_k1: 0 < k1.
+
 axiom constraints:
-  0 <= k - k1 - 1.
+  k0 + k1 <= k - 1.
 
-(* General definitions *)
-require        EF_CMA.
+op kg:int = k - k1 - 1.
+lemma leq0_kg1: 0 < kg by [].
 
-clone import EF_CMA.EF_CMA_2ROM as PSS_EF_CMA with
-  type PKS.message <- bitstring,
-  type PKS.signature <- bitstring,
-  type PKS.Gt.from <- bitstring,
-  type PKS.Gt.to <- bitstring,
-  op PKS.Gt.dsample = Dbitstring.dbitstring (k - k1  -1),
-  type PKS.Ht.from <- bitstring,
-  type PKS.Ht.to <- bitstring,
-  op PKS.Ht.dsample = Dbitstring.dbitstring k1.
-import PKS.
+op kg2:int = k - k0 - k1 - 1.
+lemma leq0_kg2: 0 <= kg2 by [].
 
-op keypairs: (pkey * skey) distr.
-axiom keypairsL: weight keypairs = 1%r.
+op k':int = k - 1.
+lemma leq0_k': 0 <= k' by [].
 
-op rsa: pkey -> bitstring -> bitstring.
-op rsa': skey -> bitstring -> bitstring.
+(** Types *)
+require AWord.
+require import ABitstring.
 
-module PSS(G:Gt.Oracle,H:Ht.Oracle): Scheme = {
-  fun g1(x:bitstring):bitstring = {
-    var r:bitstring;
-    r  = G.o(x);
-    return sub r 0 k0;
+type message = bitstring.
+
+(* Signatures *)
+type signature.
+clone import AWord as Signature with
+  type word <- signature,
+  op length <- k.
+
+(* Nonce *)
+type salt.
+clone import AWord as Salt with
+  type word <- salt,
+  op length <- k0.
+op sample_salt = Salt.Dword.dword.
+
+(* Output of H *)
+type htag.
+clone import AWord as HTag with
+  type word <- htag,
+  op length <- k1.
+op sample_htag = HTag.Dword.dword.
+
+(* Output of G *)
+type gtag.
+clone import AWord as GTag with
+  type word <- gtag,
+  op length = kg.
+op sample_gtag = GTag.Dword.dword.
+
+(* Output of G2 [G1 produces an HTag] *)
+type g2tag.
+clone import AWord as G2Tag with
+  type word <- g2tag,
+  op length = kg2.
+
+(* Domain of RSA *)
+op sample_plain: signature distr. (* Whereby we sample only with the first byte/bit set to 0 *)
+
+(** Instantiating *)
+require PKS.
+require OW.
+require RandOrcl.
+
+clone export OW as RSA with
+  type t <- signature,
+  op sample_t <- sample_plain,
+  op f_dom = (lambda (pk:pkey) (x:signature), cpTrue x),
+  op f_rng = (lambda (pk:pkey) (x:signature), cpTrue x),
+  op finv_dom = (lambda (sk:skey) (x:signature), cpTrue x),
+  op finv_rng = (lambda (sk:skey) (x:signature), cpTrue x)
+  proof f_rng_sub_finv_dom by smt,
+        finv_rng_sub_f_dom by smt,
+        f_dom_sample_t by smt.
+
+clone export RandOrcl as H with
+  type from <- message,
+  type to <- htag,
+  op dsample <- sample_htag,
+  op default = HTag.zeros.
+
+clone export RandOrcl as G with
+  type from <- htag,
+  type to <- gtag,
+  op dsample <- sample_gtag,
+  op default = GTag.zeros.
+
+clone export PKS as PKSi with
+  type pkey <- pkey,
+  type skey <- skey,
+  type message <- message,
+  type signature <- signature.
+
+(*** Defining PSS *)
+print theory GTag.
+module PSS(G:G.Oracle,H:H.Oracle): Scheme = {
+  fun init(): unit = {
+    G.init();
+    H.init();
   }
 
-  fun g2(x:bitstring):bitstring = {
-    var r:bitstring;
+  fun g1(x:htag):salt = {
+    var r:gtag;
     r  = G.o(x);
-    return sub r k0 (k - k0 - k1 - 1);
+    return Salt.from_bits (sub (to_bits r) 0 k0);
+  }
+
+  fun g2(x:htag):g2tag = {
+    var r:gtag;
+    r  = G.o(x);
+    return G2Tag.from_bits (sub (to_bits r) k0 kg2);
   }
 
   (* Keygen: make it a wrapped pop *)
@@ -53,112 +128,44 @@ module PSS(G:Gt.Oracle,H:Ht.Oracle): Scheme = {
   }
 
   (* Sign *)
-  fun sign(sk:skey, m:bitstring):bitstring = {
-    var r:bitstring;
-    var rMask:bitstring;
-    var maskedR:bitstring;
-    var w:bitstring;
-    var gamma:bitstring;
-    var y:bitstring;
+  fun sign(sk:skey, m:message):signature = {
+    var r:salt;
+    var rMask:salt;
+    var maskedR:salt;
+    var w:htag;
+    var gamma:g2tag;
+    var y:signature;
 
-    r = $Dbitstring.dbitstring(k0);
-    w  = H.o(m || r);
+    r = $sample_salt;
+    w  = H.o(m || (to_bits r));
     rMask  = g1(w);
-    maskedR = rMask ^^ r;
+    maskedR = rMask ^ r;
     gamma  = g2(w);
-    y = zeros(1) || w || maskedR || gamma;
-    return (rsa' sk m); (* For fault injection, we will later refine this; we should make it a function so it can be reasoned about separately *)
+    y = Signature.from_bits (zeros 1 || (to_bits w) || (to_bits maskedR) || (to_bits gamma));
+    return (finv sk y); (* For fault injection, we will later refine this; we should make it a function so it can be reasoned about separately *)
   }
 
   (* Verify *)
-  fun verify(pk:pkey, m:bitstring, s:bitstring):bool = {
-    var y:bitstring;
-    var w:bitstring;
-    var w':bitstring;
-    var maskedR:bitstring;
-    var gamma:bitstring;
-    var gamma':bitstring;
-    var rMask:bitstring;
-    var r:bitstring;
+  fun verify(pk:pkey, m:message, s:signature):bool = {
+    var y:signature;
+    var w:htag;
+    var w':htag;
+    var maskedR:salt;
+    var gamma:g2tag;
+    var gamma':g2tag;
+    var rMask:salt;
+    var r:salt;
     var b:bool;
 
-    y = (rsa pk s);
-    b = y.[0];
-    w = sub y 1 k1;
-    maskedR = sub y (k1 + 1) k0;
-    gamma = sub y (k1 + k0 + 1) (k - k1 - k0 - 1);
+    y = (f pk s);
+    b = (sub (to_bits y) 0 1 <> zeros 1);
+    w = HTag.from_bits (sub (to_bits y) 1 k1);
+    maskedR = Salt.from_bits (sub (to_bits y) (k1 + 1) k0);
+    gamma = G2Tag.from_bits (sub (to_bits y) (k1 + k0 + 1) kg2);
     rMask  = g1(w);
-    r = rMask ^^ maskedR;
-    w'  = H.o(m || r);
+    r = rMask ^ maskedR;
+    w'  = H.o(m || to_bits r);
     gamma'  = g2(w);
     return (w = w' /\ gamma = gamma' /\ !b);
   }
 }.
-
-module G = Gt.ROM.RO.
-module G' = Gt.WRO_Set.ARO(G).
-module H = Ht.ROM.RO.
-module H' = Ht.WRO_Set.ARO(H).
-
-section.
-declare module A:CMA {G', H', Wrap}.
-axiom losslessA (G <: Gt.ARO{A}) (H <: Ht.ARO{A}) (O <: Oracles{A}):
-  islossless O.sign => islossless H.o => islossless G.o =>
-  islossless A(G, H, O).a.
-
-module PSS_bits = PSS(G,H).
-module PSS_bors = Wrap(G,H,PSS_bits).
-module Initial = EF_CMA(G,H,PSS_bits,A).
-
-lemma terminates: islossless Initial.main.
-proof strict.
-fun.
-call (_: true ==> true);
-  first by fun.
-call (_: true ==> true); first fun.
-  call (_: true ==> true);
-    first by fun; call (_: true ==> true)=> //;
-               apply Gt.ROM.lossless_o;
-               rewrite -/(weight Gt.dsample) /Gt.dsample Dbitstring.weight_pos; smt.
-  call (_: true ==> true);
-    first by apply Ht.ROM.lossless_o;
-             rewrite -/(weight Ht.dsample) /Ht.dsample Dbitstring.weight_pos; smt.
-  wp; call (_: true ==> true);
-    first by fun; call (_: true ==> true)=> //;
-               apply Gt.ROM.lossless_o;
-               rewrite -/(weight Gt.dsample) /Gt.dsample Dbitstring.weight_pos; smt.
-  wp=> //.
-call (_: true ==> true).
-  fun true=> //.
-    by intros=> G0 H0 O; apply (losslessA G0 H0 O).
-    fun; call (_: true ==> true).
-      fun; wp; call (_: true ==> true)=> //;
-          first by fun; call (_: true ==> true)=> //;
-                     apply Gt.ROM.lossless_o=> //;
-                     rewrite -/(weight Gt.dsample) /Gt.dsample Dbitstring.weight_pos; smt.
-        wp; call (_: true ==> true)=> //;
-          first by fun; call (_: true ==> true)=> //;
-                     apply Gt.ROM.lossless_o=> //;
-                     rewrite -/(weight Gt.dsample) /Gt.dsample Dbitstring.weight_pos; smt.
-        call (_: true ==> true)=> //;
-          first by apply Ht.ROM.lossless_o=> //;
-                   rewrite -/(weight Ht.dsample) /Ht.dsample Dbitstring.weight_pos; smt.
-        by rnd=> // _; rewrite -/cpTrue -/(weight (Bitstring.Dbitstring.dbitstring k0))
-                               Bitstring.Dbitstring.weight_pos // leq0_k0.
-      wp=> //.
-    fun; if; try wp=> //.
-      call (_: true ==> true); try wp=> //;
-        first by apply Ht.ROM.lossless_o=> //;
-                 rewrite -/(weight Ht.dsample) /Ht.dsample Dbitstring.weight_pos; smt.
-    fun; if; try wp=> //.
-      call (_: true ==> true); try wp=> //;
-        first by apply Gt.ROM.lossless_o=> //;
-                 rewrite -/(weight Gt.dsample) /Gt.dsample Dbitstring.weight_pos; smt.
-call (_: true ==> true)=> //; fun;
-  call (_: true ==> true);
-    first fun; rnd=> // _; apply keypairsL.
-  wp; call (_: true ==> true);
-    first apply Gt.ROM.lossless_init.
-  wp; call (_: true ==> true)=> //;
-    apply Ht.ROM.lossless_init.
-qed.
