examples/AWord.ec
@@ -1,0 +1,28 @@
+require import Int.
+
+type word.
+
+const length:int.
+axiom leq0_length: 0 <= length.
+
+op zeros: word.
+
+op ( ^ ): word -> word -> word.
+
+require import ABitstring.
+op to_bits: word -> bitstring.
+op from_bits: bitstring -> word.
+
+axiom length_to_bits w:
+  `|to_bits w| = length.
+axiom can_from_to w:
+  from_bits (to_bits w) = w.
+axiom pcan_to_from (b:bitstring):
+  `|b| = length =>
+  to_bits (from_bits b) = b.
+
+theory Dword.
+  require import Distr.
+
+  op dword: word distr.
+end Dword.
